wip

src/hashtable.v
@@ -1,39 +1,57 @@
 Require Import Coq.Array.PArray.
 Require Import Coq.Init.Nat.
+Require Import ZArith.
 Require Import Bool.
+Require Import Lia.
 Require Import Coq.Lists.List.
 Import ListNotations.
-Require Import Coq.Numbers.Cyclic.Int63.Sint63.
-Require Import Coq.Numbers.Cyclic.Int63.PrimInt63.
+Require Import Coq.Numbers.Cyclic.Int63.Uint63.
+(* Require Import Coq.Numbers.Cyclic.Int63.PrimInt63. *)
 
-
-Let array := make 6 1%nat.
-
-Let array2 := set array 2 2%nat.
-
-Compute (get array2 2).
-
-Open Scope int63_scope.
-Open Scope sint63_scope.
+Open Scope uint63_scope.
+Print int.
+Check to_Z.
 
 Section Hashtable.
   Context {A B: Set}.
   Variable eq: A -> A -> bool.
   Variable eq_spec: forall x y : A, reflect (x = y) (eq x y).
-
   Variable hash: A -> int.
+
+  Lemma eq_true:
+    forall (k1 k2 : A), k1 = k2 -> eq k1 k2 = true.
+  Proof.
+    intros k1 k2 H.
+    now case eq_spec.
+  Qed.
+
+  Lemma eq_false:
+    forall (k1 k2 : A), k1 <> k2 -> eq k1 k2 = false.
+  Proof.
+    intros k1 k2 H.
+    now case eq_spec.
+  Qed.
+
+  Lemma eq_refl:
+    forall (k : A), eq k k = true.
+  Proof.
+    intros k.
+    now case eq_spec.
+  Qed.
 
   Definition bucket := list (A * B).
   Definition table := PArray.array bucket.
   
-  (* Inductive hashtab : Set := hash_tab : int -> table -> hashtab. *)
-  Record t : Set := hash_tab { capacity : int; size : int; hashtab : table }.
+  Record t : Set := hash_tab { 
+    size : int;
+    hashtab : table; 
+  }.
 
-  Fixpoint power_2_above' (n: nat) (x p :int) {struct n} : int :=
+  Fixpoint power_2_above' (n: nat) (x p: int) {struct n} : int :=
     match n with
-    | O   => p
-    | S n => if (p <? x) 
-             then power_2_above' n x (p * 2)
+    | O    => p
+    | S n' => if (p <? x) 
+             then power_2_above' n' x (p * 2)
              else p
     end.
   
@@ -42,16 +60,41 @@ Section Hashtable.
 
   Definition create (initial_size: int) : t :=
     let size := power_2_above initial_size 16 in
-    hash_tab size 0 (make size []).
+    let h := make size [] in
+    hash_tab 0 h.
 
-  Definition key_index (h: t) (k: A) :=
+
+  Definition key_index (h: t) (k: A) : int :=
     (hash k) land (PArray.length (hashtab h) - 1).
 
-  Definition add (h: t) (key: A) (v: B) :=
+  Definition get_bucket (h: t) (k: A) : bucket :=
+    if PArray.length (hashtab h) =? 0 then
+      []
+    else 
+      (hashtab h).[key_index h k].
+
+  Definition resize_heurisitic (h: t) : bool :=
+    PArray.length (hashtab h) =? 0.
+
+  Definition resize (h: t): t :=
+    if PArray.length (hashtab h) =? 0 then 
+      hash_tab 0 (make 16 [])
+    else h.
+
+  Lemma length_resize:
+    forall (h: t),
+    (0 < to_Z (PArray.length (hashtab (resize h))))%Z.
+  Proof.
+    admit.
+  Admitted.
+
+  Definition add (h: t) (key: A) (v: B) : t :=
+    let h := resize h in
     let tab := hashtab h in
     let i := key_index h key in
     let bucket := get tab i in
-    set tab i ((key, v) :: bucket).
+    let new := (key, v) :: tab.[i] in
+    hash_tab (size h + 1) tab.[i<-new].
 
   Fixpoint find_rec (l: bucket) (key: A) : option B :=
     match l with
@@ -59,11 +102,106 @@ Section Hashtable.
     | (k', v) :: l' => if eq k' key then Some v else find_rec l' key
     end.
 
-  Definition find (key: A) (h: t) : option B :=
-    let i := key_index h key in
-    let bucket := get (hashtab h) i in
+  Fixpoint find_all_rec (l: bucket) (key: A) (acc: list B): list B :=
+    match l with
+    | [] => List.rev' acc
+    | (k', v) :: l' => 
+        if eq k' key 
+        then find_all_rec l' key (v :: acc)
+        else find_all_rec l' key acc
+    end.
+
+  Fixpoint find_all_rec' (l: bucket) (key: A) : list B :=
+    match l with
+    | [] => []
+    | (k', v) :: l' => 
+        if eq k' key 
+        then v :: find_all_rec' l' key
+        else find_all_rec' l' key
+    end.
+
+  Lemma find_all_rec_correct:
+    forall (l: bucket) (key: A),
+    find_all_rec l key [] = find_all_rec' l key.
+  Proof.
+    intros l key. 
+    change (find_all_rec l key [] = rev [] ++ find_all_rec' l key).
+    generalize (nil : list B). induction l.
+    + intros acc. simpl. apply rev_append_rev.
+    + intros acc. simpl. destruct a. case eq.
+      rewrite IHl. simpl. rewrite <- app_assoc. easy.
+      apply IHl.
+  Qed.
+
+  Definition find (h: t) (key: A) : option B :=
+    let bucket := get_bucket h key in
     find_rec bucket key.
+
+  Definition find_all (h: t) (key: A) : list B :=
+    find_all_rec (get_bucket h key) key [].
+
+  Lemma find_all_resize:
+    forall (h: t) (k: A),
+    find_all (resize h) k = find_all h k.
+  Proof.
+    intros h k. unfold resize, find_all, get_bucket.
+    case (PArray.length (hashtab h) =? 0) eqn:Heqb.
+    simpl eqb. cbn iota. unfold hashtab.
+    now rewrite get_make.
+    now rewrite Heqb.
+  Qed.
+
+  Theorem hempty:
+    forall (k: A) (size: int), find (create size) k = None.
+  Proof. Admitted.
+  (*   intros k i. unfold create, find, get_bucket. simpl. *)
+  (*   rewrite length_make. *)
+  (*   now rewrite get_make. *)
+  (* Qed. *)
+
+  Lemma key_index_eq:
+    forall (h1 h2: t) (k: A), 
+    PArray.length (hashtab h1) = PArray.length (hashtab h2) ->
+    key_index h1 k = key_index h2 k.
+  Proof.
+    intros h1 h2 k H. unfold key_index.
+    now rewrite H.
+  Qed.
+
+  Theorem dadd:
+    forall (k: A) (v: B) (h: t),
+    find_all (add h k v) k = v::(find_all h k).
+  Proof.
+    intros k v h. rewrite <- (find_all_resize h).
+    unfold find_all.
+    rewrite 2!find_all_rec_correct.
+    unfold get_bucket.
+    rewrite 2!eqb_false_complete.
+    rewrite (key_index_eq (add h k v) (resize h)).
+    unfold add; simpl. rewrite get_set_same.
+    simpl. rewrite eq_refl. easy.
+    admit.
+    unfold add; simpl. apply length_set.
+  Admitted.
 
 End Hashtable.
 
+Module Type Hash_type.
+  Variable A: Set.
+  Variable eq: A -> A -> bool.
+  Variable eq_spec: forall x y : A, reflect (x = y) (eq x y).
+  Variable hash: A -> int.
+End Hash_type.
+
+Module HashTable (T: Hash_type).
+  Definition t := @t T.A.
+  Definition create (B: Set) (initial_size: int) : t B :=
+    create initial_size.
+
+  Definition add {B: Set} (h: t B) (key: T.A) (v: B) :=
+    add T.hash h key v.
+
+  Definition find {B: Set} (h: t B) (key: T.A): option B :=
+    find T.eq T.hash key h.
+End HashTable.
 
